src/proof/well_formed.v
@@ -37,11 +37,6 @@ Definition pod_well_formed (pod: v1.Pod.t) : iProp Σ :=
   "#pod_spec_well_formed" ∷ pod_spec_well_formed pod.(v1.Pod.Spec') ∗
   "#pod_status_well_formed" ∷ pod_status_well_formed pod.(v1.Pod.Status').
 
-Definition pod_nn_well_formed (pod: v1.Pod.t) (namespace name: go_string) : iProp Σ :=
-  "%namespace_match" ∷ ⌜ pod.(v1.Pod.ObjectMeta').(v1.ObjectMeta.Namespace') = namespace ⌝ ∗
-  "%name_match" ∷ ⌜ pod.(v1.Pod.ObjectMeta').(v1.ObjectMeta.Name') = name ⌝ ∗
-  "#pod_well_formed" ∷ pod_well_formed pod.
-
 Definition object_meta_to_create_well_formed (m: v1.ObjectMeta.t) : iProp Σ :=
   "%generatename_not_empty_if_name_empty" ∷ ⌜ m.(v1.ObjectMeta.Name') = ""%go → m.(v1.ObjectMeta.GenerateName') ≠ ""%go ⌝.
 
@@ -67,17 +62,17 @@ Definition replicaset_well_formed (rs: v1.ReplicaSet.t) : iProp Σ :=
   object_meta_well_formed rs.(v1.ReplicaSet.ObjectMeta') ∗
   ∃ (v: w32), rs.(v1.ReplicaSet.Spec').(v1.ReplicaSetSpec.Replicas') ↦□ v ∗ ⌜ 0 ≤ sint.Z v ⌝.
 
-Definition replicaset_nn_well_formed (rs: v1.ReplicaSet.t) (namespace name: go_string) : iProp Σ :=
-  ⌜ rs.(v1.ReplicaSet.ObjectMeta').(v1.ObjectMeta.Namespace') = namespace ⌝ ∗
-  ⌜ rs.(v1.ReplicaSet.ObjectMeta').(v1.ObjectMeta.Name') = name ⌝ ∗
-  replicaset_well_formed rs.
-
 Lemma well_formed_preserved_by_deepcopy_ReplicaSet rs1 rs2 namespace name:
   deepcopy_ReplicaSet rs1 rs2 -∗
-    replicaset_nn_well_formed rs1 namespace name -∗
+    ⌜ rs1.(v1.ReplicaSet.ObjectMeta').(v1.ObjectMeta.Namespace') = namespace ⌝ -∗
+    ⌜ rs1.(v1.ReplicaSet.ObjectMeta').(v1.ObjectMeta.Name') = name ⌝ -∗
+    replicaset_well_formed rs1 -∗
       deepcopy_ReplicaSet rs1 rs2 ∗
-      replicaset_nn_well_formed rs1 namespace name ∗
-      replicaset_nn_well_formed rs2 namespace name.
+      ⌜ rs1.(v1.ReplicaSet.ObjectMeta').(v1.ObjectMeta.Namespace') = namespace ⌝ ∗
+      ⌜ rs1.(v1.ReplicaSet.ObjectMeta').(v1.ObjectMeta.Name') = name ⌝ ∗
+      ⌜ rs2.(v1.ReplicaSet.ObjectMeta').(v1.ObjectMeta.Namespace') = namespace ⌝ ∗
+      ⌜ rs2.(v1.ReplicaSet.ObjectMeta').(v1.ObjectMeta.Name') = name ⌝ ∗
+      replicaset_well_formed rs2.
 Proof.
 Admitted.
 
